fix to pointer casts

refinedVST/typing/own.v
@@ -321,46 +321,55 @@ Section own.
   Definition type_assert_ptr_own_inst := [instance type_assert_ptr_own].
   Global Existing Instance type_assert_ptr_own_inst.
 
-  Definition is_cast_case_pointer cty:=
-    match cty with
-    | Tint _ _ _ => if Archi.ptr64 then false else true
-    | Tlong _ _ => if Archi.ptr64 then true else false
-    | Tpointer _ _ | Tarray _ _ _ | Tfunction _ _ _  
-      => true
+  (* Definition is_cast_to_pointer ty_from ty_to:=
+    match ty_to with
+    | Tpointer _ _ =>
+      match ty_from with
+      | Tint _ _ _ => if Archi.ptr64 then false else true
+      | Tlong _ _ => if Archi.ptr64 then true else false
+      | Tpointer _ _ | Tarray _ _ _ | Tfunction _ _ _  
+        => true
+      | _ => false
+      end
     | _ => false
-    end.
+    end. *)
   
-  Lemma is_cast_case_pointer_correct cty_from cty':
-    is_cast_case_pointer cty_from <->
+  (* Lemma is_cast_to_pointer_correct cty_from cty':
+    is_cast_to_pointer cty_from (tptr cty') <->
     classify_cast cty_from (tptr cty')  = cast_case_pointer.
-  Proof. intros; destruct cty_from, cty'; done. Qed.
+  Proof. intros; destruct cty_from, cty'; done. Qed. *)
 
-  Definition cast_int_ptr v cty :=
+  (* casting a value v from cty to (tptr _). *)
+  Definition cast_to_tptr v cty :=
     match v, cty with
-    | Vint _, Tint _ _ _ => if Archi.ptr64 then None else Some $ Vint Int.zero
-    | Vlong _, Tlong _ _ => if Archi.ptr64 then Some v else Some $ Vlong Int64.zero
-    | Vptr _ _, Tlong _ _ => 
-      (* don't support Vlong and Vptr for now *)
-      Some v 
+    | Vint n, Tint _ si _ => 
+      if Archi.ptr64
+      then (* cast_case_i2l si *)
+        Some (Vlong (cast_int_long si n))
+      else Some v
+    | Vlong n, Tlong _ _ =>
+      if Archi.ptr64
+      then Some v
+      else (* cast_case_l2i I32 Unsigned *) 
+        Some(Vint (cast_int_int I32 Unsigned (Int.repr (Int64.unsigned n))))
+    | Vptr _ _, Tlong _ _
+    | Vptr _ _, Tpointer _ _
+    | Vptr _ _, Tarray _ _ _
+    | Vptr _ _, Tfunction _ _ _  =>
+      Some v
     | _, _ => None
    end.
   
   Lemma cast_int_ptr_sem_cast v v' ty ty2 m:
-    cast_int_ptr v ty = Some v'->
+    cast_to_tptr v ty = Some v'->
     Cop.sem_cast v ty (tptr ty2) m = Some v'.
   Proof.
-    intros. destruct v, ty; done.
+    intros. destruct v, ty eqn:?; done.
   Qed.
 
-  (* Vlong casted to tptr is still Vlong. *)
-  Remark Vlong_cast m:
-    Cop.sem_cast (Vlong Int64.one) tlong (tptr tvoid) m = Some (Vlong Int64.one).
-  Proof. rewrite /sem_cast /=. change Archi.ptr64 with true; done. Qed.
-
-  Lemma type_cast_int_ptr_cast_case_pointer f e ot T
-   `{!TCDone $ is_cast_case_pointer (typeof e) = true} :
+  Lemma type_cast_int_ptr_cast_case_pointer f e ot T:
        typed_val_expr ge f e (λ v ty0,
-       ∃ v', <affine> ⌜Some v' = cast_int_ptr v (typeof e)⌝ ∗
+       ∃ v', <affine> ⌜Some v' = cast_to_tptr v (typeof e)⌝ ∗
       (⎡v ◁ᵥₐₗ|typeof e| ty0⎤ -∗
       <affine> ⌜is_pointer_or_null v'⌝ ∗ T v' (value (tptr ot) v')))
     ⊢ typed_val_expr ge f (Ecast e (tptr ot)) T.
@@ -381,52 +390,7 @@ Section own.
     rewrite andb_false_r //.
   Qed.
   Definition type_cast_int_ptr_cast_case_pointer_inst := [instance type_cast_int_ptr_cast_case_pointer].
-  (* FIXME  Global Existing Instance type_cast_int_ptr_cast_case_pointer_inst | 50. *)
-
-  Definition is_cast_case_i2l cty:=
-  match cty with
-  | Tint _ _ _ => if Archi.ptr64 then true else false
-  | _ => false
-  end.
-
-  Definition cast_int_i2l v cty :=
-    match v, cty with
-    | Vint n, Tint _ si _ => Some(Vlong (cast_int_long si n))
-    | _, _ => None
-    end.
-
-  Lemma cast_int_i2l_sem_cast v v' ty ty2 m:
-    cast_int_i2l v ty = Some v'->
-    Cop.sem_cast v ty (tptr ty2) m = Some v'.
-  Proof.
-    intros. destruct v, ty; done.
-  Qed.
-  
-  Lemma type_cast_int_ptr_cast_case_i2l f e ot T
-   `{!TCDone $ is_cast_case_i2l (typeof e) = true} :
-       typed_val_expr ge f e (λ v ty0,
-       ∃ v', <affine> ⌜Some v' = cast_int_i2l v (typeof e)⌝ ∗
-      (⎡v ◁ᵥₐₗ|typeof e| ty0⎤ -∗
-      <affine> ⌜is_pointer_or_null v'⌝ ∗ T v' (value (tptr ot) v')))
-    ⊢ typed_val_expr ge f (Ecast e (tptr ot)) T.
-      Proof.
-    intros; iIntros "He %Φ HΦ".
-    iApply wp_cast0.
-    iApply "He".
-    iIntros (v ?) "own_v (%v' & % & HT)".
-    iDestruct ("HT" with "own_v") as "(% & HT)".
-    iExists v'; subst; iSplit.
-    { iPureIntro; intros. apply cast_int_i2l_sem_cast. done. }
-    iApply ("HΦ" with "[] HT").
-    unfold value; simpl_type.
-    iPureIntro; split3; try done.
-    split; last done.
-    rewrite value_fits_eq /=.
-    intros ?; simpl.
-    rewrite andb_false_r //.
-  Qed.
-  Definition type_cast_int_ptr_cast_case_i2l_inst := [instance type_cast_int_ptr_cast_case_i2l].
-  (* FIXME Global Existing Instance type_cast_int_ptr_cast_case_pointer_inst | 50. *)
+  (* Global Existing Instance type_cast_int_ptr_cast_case_pointer_inst | 50. *)
 
 (*  Lemma type_copy_aid v a it l β ty T:
     (l ◁ₗ{β} ty -∗
